cp

examples/low-level/crypto/Crypto.WIP.fst
@@ -309,158 +309,122 @@ let finish_after_mac h0 h3 i st n aadlen aad plainlen plain cipher_tagged ak l a
   end
   else FStar.Classical.move_requires (Buffer.lemma_reveal_modifies_1 tag h3) h4
   
-(* val encrypt:  *)
-(*   i: id -> st:state i Writer ->  *)
-(*   n: Cipher.iv (alg i) -> *)
-(*   aadlen: UInt32.t {aadlen <=^ aadmax} ->  *)
-(*   aad: lbuffer (v aadlen) ->  *)
-(*   plainlen: UInt32.t {plainlen <> 0ul /\ safelen i (v plainlen) 1ul} ->  *)
-(*   plain: plainBuffer i (v plainlen) ->  *)
-(*   cipher:lbuffer (v plainlen + v (Spec.taglen i))  *)
-(*   {  *)
-(*     Buffer.disjoint aad cipher /\ *)
-(*     Buffer.disjoint (Plain.as_buffer plain) aad /\ *)
-(*     Buffer.disjoint (Plain.as_buffer plain) cipher /\ *)
-(*     HH.disjoint (Buffer.frameOf (Plain.as_buffer plain)) st.log_region /\ *)
-(*     HH.disjoint (Buffer.frameOf cipher) st.log_region /\ *)
-(*     HH.disjoint (Buffer.frameOf aad) st.log_region *)
-(*   } *)
-(*   ->   *)
-(*   //STL -- should be STL eventually, but this requires propagation throughout the library *)
-(*   ST unit *)
-(*   (requires (fun h ->  *)
-(*     let prf_rgn = st.prf.rgn in *)
-(*     my_inv st h /\ *)
-(*     Buffer.live h aad /\ *)
-(*     Buffer.live h cipher /\  *)
-(*     Plain.live h plain /\ *)
-(*     (prf i ==> none_above ({iv=n; ctr=0ul}) st.prf h) // The nonce must be fresh! *)
-(*    )) *)
-(*   (ensures (fun h0 _ h1 ->  *)
-(*     //TODO some "heterogeneous" modifies that also records updates to logs and tables *)
-(*     HS.modifies (Set.union (Set.singleton st.log_region) *)
-(* 			   (Set.singleton (Buffer.frameOf cipher))) h0 h1 /\ *)
-(*     (\* Buffer.m_ref (Buffer.frameOf cipher) !{Buffer.modifies_1 cipher h0 h1 /\  *\) *)
-(*     Buffer.live h1 aad /\ *)
-(*     Buffer.live h1 cipher /\  *)
-(*     Plain.live h1 plain /\ *)
-(*     my_inv st h1 /\ *)
-(*     (safeId i ==> ( *)
-(*       let aad = Buffer.as_seq h1 aad in *)
-(*       let p = Plain.sel_plain h1 plainlen plain in *)
-(*       let c = Buffer.as_seq h1 cipher in *)
-(*       HS.sel h1 st.log == SeqProperties.snoc (HS.sel h0 st.log) (Entry n aad (v plainlen) p c))) *)
-(*    )) *)
-
-(* let encrypt i st n aadlen aad plainlen plain cipher_tagged = *)
-(*   let h0 = get() in *)
-(*   assume (HS (is_stack_region h0.tip)); //TODO: remove this once we move all functions to STL *)
-(*   assume (HS (HH.disjoint h0.tip st.prf.mac_rgn)); //DO we need disjointness or will disequality do? *)
-(*   let x = PRF({iv = n; ctr = 0ul}) in // PRF index to the first block *)
-(*   let ak = PRF.prf_mac i st.prf x in  // used for keying the one-time MAC   *)
-(*   let h1 = get () in  *)
-(*   assert (HS.modifies_ref st.prf.mac_rgn TSet.empty h0 h1); *)
-(*   let cipher = Buffer.sub cipher_tagged 0ul plainlen in *)
-(*   let tag = Buffer.sub cipher_tagged plainlen (Spec.taglen i) in *)
-(*   let y = PRF.incr i x in *)
-(*   //calling this lemma allows us to complete the proof without using any fuel; *)
-(*   //which makes things a a bit faster *)
-(*   counterblocks_emp i st.prf.mac_rgn y (v plainlen) 0 *)
-(*       (Plain.sel_plain h1 plainlen plain) (Buffer.as_seq h1 cipher); *)
-(*   counter_enxor i st.prf y plainlen plainlen plain cipher h1; *)
-(*   // Compute MAC over additional data and ciphertext *)
-(*   let h2 = get () in *)
-(*   FStar.Classical.move_requires (Buffer.lemma_reveal_modifies_1 cipher h1) h2; *)
-(*   assert (HS.modifies_ref st.prf.mac_rgn TSet.empty h0 h2); *)
-(*   lemma_frame_find_mac #i #(v plainlen) st.prf y cipher h1 h2; *)
-(*   intro_refines_one_entry_no_tag #i st n (v plainlen) plain cipher_tagged h0 h1 h2; //we have pre_refines_one_entry here *)
-(*   assert (Buffer.live h1 aad); //seem to need this hint *)
-(*   let l, acc = accumulate ak aadlen aad plainlen cipher in *)
-(*   let h3 = get() in *)
-(*   Buffer.lemma_reveal_modifies_0 h2 h3; *)
-(*   assert (HS.modifies_ref st.prf.mac_rgn TSet.empty h0 h3); *)
-(*   frame_pre_refines_0 i st n (v plainlen) plain cipher_tagged h0 h2 h3; *)
-(*   assert (Buffer.live h2 aad); //seem to need this hint *)
-(*   assert (Buffer.live h3 aad); //seem to need this hint *)
-(*   Buffer.lemma_reveal_modifies_0 h2 h3; *)
-(*   MAC.mac ak l acc tag; *)
-(*   let h4 = get () in *)
-(*   FStar.Classical.move_requires (Buffer.lemma_reveal_modifies_1 tag h3) h4; *)
-(*   modifies_fresh_empty i n st.prf.mac_rgn ak h0 h3 h4; *)
-(*   assert (safeId i ==> HS.modifies_ref st.prf.mac_rgn TSet.empty h0 h4); *)
-(*   frame_pre_refines i st n (v plainlen) plain cipher_tagged h0 h3 h4; *)
-(*   intro_mac_refines i st n aad plain cipher_tagged h4; *)
-(*   pre_refines_to_refines i st n aadlen aad (v plainlen) plain cipher_tagged h0 h4; *)
-(*   extend_refines_aux i st n aadlen aad (v plainlen) plain cipher_tagged h0 h4; *)
-(*   refines_to_inv i st n aadlen aad plainlen plain cipher_tagged; *)
-(*   (\* assert (my_inv st h4); *\) *)
-(*   admit() *)
-  
-
-
-
-  (*   live h0 tag /\ live h0 st.s /\ *)
-  (*   disjoint acc st.s /\ disjoint tag acc /\ disjoint tag st.r /\ disjoint tag st.s /\ *)
-  (*   acc_inv st l acc h0 /\ *)
-  (*   (mac_log ==> m_contains (ilog st.log) h0) /\ *)
-  (*   (mac_log /\ safeId (fst i) ==> m_sel h0 (ilog st.log) == None))) *)
-  (* (ensures (fun h0 _ h1 -> *)
-  (*   live h0 st.s /\  *)
-  (*   live h0 st.r /\  *)
-  (*   live h1 tag /\ ( *)
-  (*   if mac_log then *)
-  (*     mods_2 [Ref (as_hsref (ilog st.log)); Ref (Buffer.content tag)] h0 h1 /\ *)
-  (*     Buffer.modifies_buf_1 (Buffer.frameOf tag) tag h0 h1 /\ *)
-  (*     HS.modifies_ref st.region !{HS.as_ref (as_hsref (ilog st.log))} h0 h1 /\ *)
-  (*     m_contains (ilog st.log) h1 /\ ( *)
-  (*     let mac = mac_1305 l (sel_elem h0 st.r) (sel_word h0 st.s) in *)
-  (*     mac == little_endian (sel_word h1 tag) /\ *)
-  (*     m_sel h1 (ilog st.log) == Some (l, sel_word h1 tag)) *)
-  (*   else Buffer.modifies_1 tag h0 h1))) *)
-
-  
-  (* let _ = *)
-  (*   let tab = HS.sel h4 (itable i st.prf) in *)
-  (*   match PRF.find_mac tab x with *)
-  (*   | None -> assert False *)
-  (*   | Some mac_st -> assert(mac_st == ak) in *)
-  (* admit() *)
-  
-
-  (* admit() *)
-
+val encrypt:
+  i: id -> st:state i Writer ->
+  n: Cipher.iv (alg i) ->
+  aadlen: UInt32.t {aadlen <=^ aadmax} ->
+  aad: lbuffer (v aadlen) ->
+  plainlen: UInt32.t {plainlen <> 0ul /\ safelen i (v plainlen) 1ul} ->
+  plain: plainBuffer i (v plainlen) ->
+  cipher_tagged:lbuffer (v plainlen + v (Spec.taglen i))
+  {
+    Buffer.disjoint aad cipher_tagged /\
+    Buffer.disjoint (Plain.as_buffer plain) aad /\
+    Buffer.disjoint (Plain.as_buffer plain) cipher_tagged /\
+    HH.disjoint (Buffer.frameOf (Plain.as_buffer plain)) st.log_region /\
+    HH.disjoint (Buffer.frameOf cipher_tagged) st.log_region /\
+    HH.disjoint (Buffer.frameOf aad) st.log_region
+  }
+  ->
+  //STL -- should be STL eventually, but this requires propagation throughout the library
+  ST unit
+  (requires (fun h ->
+    let prf_rgn = st.prf.rgn in
+    my_inv st h /\
+    Buffer.live h aad /\
+    Buffer.live h cipher_tagged /\
+    Plain.live h plain /\
+    (prf i ==> none_above ({iv=n; ctr=0ul}) st.prf h) // The nonce must be fresh!
+   ))
+  (ensures (fun h0 _ h5 ->
+  	           Buffer.live h5 aad /\
+		   Buffer.live h5 cipher_tagged /\
+		   Plain.live h5 plain /\
+		   my_inv st h5 /\
+		   HS.modifies_transitively (as_set [st.log_region; Buffer.frameOf cipher_tagged]) h0 h5 /\ (
+		   safeId i ==>  (
+		     let aad = Buffer.as_seq h5 aad in
+		     let p = Plain.sel_plain h5 plainlen plain in
+		     let c = Buffer.as_seq h5 cipher_tagged in
+		     HS.sel h5 st.log == SeqProperties.snoc (HS.sel h0 st.log) (Entry n aad (v plainlen) p c)))))
+    (* Buffer.m_ref (Buffer.frameOf cipher) !{Buffer.modifies_1 cipher h0 h1 /\  *) 
+unfold let mac_ensures_2 (i:MAC.id) (st:MAC.state i) (l:MAC.itext) (acc:MAC.accB i) (tag:MAC.tagB) 
+		(h0:mem) (h1:mem) = 
+    let open FStar.Buffer in
+    let open Crypto.Symmetric.Bytes in
+    let open Crypto.Symmetric.Poly1305 in
+    let open Crypto.Symmetric.Poly1305.Spec in
+    let open Crypto.Symmetric.Poly1305.MAC in
+    live h0 st.s /\ 
+    live h0 st.r /\ 
+    live h1 tag /\ (
+    if mac_log then
+      HS.modifies (as_set [st.region; Buffer.frameOf tag]) h0 h1 /\
+      mods_2 [HS.Ref (as_hsref (ilog st.log)); HS.Ref (Buffer.content tag)] h0 h1 /\
+      Buffer.modifies_buf_1 (Buffer.frameOf tag) tag h0 h1 /\
+      HS.modifies_ref st.region !{HS.as_ref (as_hsref (ilog st.log))} h0 h1 /\
+      m_contains (ilog st.log) h1 /\ (
+      let mac = mac_1305 l (sel_elem h0 st.r) (sel_word h0 st.s) in
+      mac == little_endian (sel_word h1 tag) /\
+      m_sel h1 (ilog st.log) == Some (l, sel_word h1 tag))
+    else Buffer.modifies_1 tag h0 h1)
     
-      (*  admit() in *)
-       
-      (* let c = Buffer.as_seq h4 cipher in *)
-      (* let ad = Buffer.as_seq h4 aad in *)
-      (* assume (l == field_encode i ad #plainlen c); *)
-      (* intro_mac_refines i st n aad plain cipher_tagged h4 in *)
-
-  (*   () in  *)
-  (* admit() *)
-  
-
-
-  (* assume (mac_refines i st.prf.mac_rgn (v plainlen) (as_seq h4 aad) (Plain.sel_plain h4 plainLen plain) (Buffer.as_seq tag) _ h4); *)
-  (* assume false *)
-
-  
-  (* let h4 = get () in  *)
-  (* assume (HS (modifies (Set.union (Set.singleton (Buffer.frameOf tag)) *)
-  (* 				  (Set.singleton st.prf.mac_rgn)) h3 h4)); *)
-  (* assume (Buffer.modifies_buf_1 (Buffer.frameOf tag) tag h3 h4); *)
-  (* let _ =  *)
-  (*   let mod_set = MAC (if mac_log then !{HS.as_ref (as_hsref (MAC.ilog ak.log))} else !{}) in *)
-  (*   assume (HS (modifies_ref st.prf.mac_rgn mod_set h3 h4)) in *)
-  (* if safeId i *)
-  (* then begin *)
-  (*   let aad = temp_to_seq aad in *)
-  (*   let p = temp_get_plain plain in *)
-  (*   let c = temp_to_seq cipher in *)
-  (*   assume false; *)
-  (*   let entry = Entry n aad (v plainlen) p c in *)
-  (*   st.log := SeqProperties.snoc !st.log entry *)
-  (* end; *)
-  (* assume false *)
-  (* pop_frame() *)
+let mac_wrapper (#i:MAC.id) (st:MAC.state i) (l:MAC.itext) (acc:MAC.accB i) (tag:MAC.tagB)
+  : ST unit
+    (requires (fun h0 ->
+      let open Crypto.Symmetric.Poly1305.MAC in
+      Buffer.live h0 tag /\ 
+      Buffer.live h0 st.s /\
+      Buffer.disjoint acc st.s /\ 
+      Buffer.disjoint tag acc /\ 
+      Buffer.disjoint tag st.r /\ 
+      Buffer.disjoint tag st.s /\
+      MAC.acc_inv st l acc h0 /\
+      (MAC (mac_log ==> m_contains (ilog st.log) h0)) /\
+      (MAC (mac_log /\ safeId (fst i) ==> m_sel h0 (ilog st.log) == None))))
+  (ensures (fun h0 _ h1 -> mac_ensures i st l acc tag h0 h1))
+ = let h0 = get () in
+   MAC.mac #i st l acc tag;
+   let h1 = get () in
+   assume (HS.modifies (as_set [MAC st.region; Buffer.frameOf tag]) h0 h1);
+   admit()
+   
+#reset-options "--z3timeout 1000 --initial_fuel 0 --max_fuel 0 --initial_ifuel 0 --max_ifuel 0"
+let encrypt i st n aadlen aad plainlen plain cipher_tagged =
+  let h0 = get() in
+  assume (HS (is_stack_region h0.tip)); //TODO: remove this once we move all functions to STL
+  assume (HS (HH.disjoint h0.tip st.prf.mac_rgn)); //DO we need disjointness or will disequality do?
+  let x = PRF({iv = n; ctr = 0ul}) in // PRF index to the first block
+  let ak = PRF.prf_mac i st.prf x in  // used for keying the one-time MAC
+  let h1 = get () in
+  assert (HS.modifies_ref st.prf.mac_rgn TSet.empty h0 h1);
+  let cipher = Buffer.sub cipher_tagged 0ul plainlen in
+  let tag = Buffer.sub cipher_tagged plainlen (Spec.taglen i) in
+  let y = PRF.incr i x in
+  //calling this lemma allows us to complete the proof without using any fuel;
+  //which makes things a a bit faster
+  counterblocks_emp i st.prf.mac_rgn y (v plainlen) 0
+      (Plain.sel_plain h1 plainlen plain) (Buffer.as_seq h1 cipher);
+  counter_enxor i st.prf y plainlen plainlen plain cipher h1;
+  // Compute MAC over additional data and ciphertext
+  let h2 = get () in
+  FStar.Classical.move_requires (Buffer.lemma_reveal_modifies_1 cipher h1) h2;
+  assert (HS.modifies_ref st.prf.mac_rgn TSet.empty h0 h2);
+  lemma_frame_find_mac #i #(v plainlen) st.prf y cipher h1 h2;
+  intro_refines_one_entry_no_tag #i st n (v plainlen) plain cipher_tagged h0 h1 h2; //we have pre_refines_one_entry here
+  assert (Buffer.live h1 aad); //seem to need this hint
+  let l, acc = accumulate ak aadlen aad plainlen cipher in
+  //Establishing the pre-conditions of MAC.mac
+  let h3 = get() in
+  assume (HS.modifies_transitively (as_set [st.log_region; Buffer.frameOf cipher_tagged]) h0 h3); //TODO: prove this!
+  Buffer.lemma_reveal_modifies_0 h2 h3;
+  assert (HS.modifies_ref st.prf.mac_rgn TSet.empty h0 h3);
+  frame_pre_refines_0 i st n (v plainlen) plain cipher_tagged h0 h2 h3;
+  assert (Buffer.live h2 aad); //seem to need this hint
+  assert (Buffer.live h3 aad); //seem to need this hint
+  Buffer.lemma_reveal_modifies_0 h2 h3;
+  //MAC
+  mac_wrapper #(i,n) ak l acc tag;
+  //Some ideal and proof steps, to finish up
+  finish_after_mac h0 h3 i st n aadlen aad plainlen plain cipher_tagged ak l acc tag;
+  admit()
